wip low-level implementation of Merkle tree

examples/low-level/merkletree/MerkleTree.Low.fst
@@ -9,6 +9,7 @@ open LowStar.Modifies
 open LowStar.BufferOps
 open FStar.Seq
 open FStar.Integers
+open FStar.BitVector
 
 module List = FStar.List.Tot
 module HS = FStar.HyperStack
@@ -20,108 +21,247 @@ module S = FStar.Seq
 
 let root = Monotonic.HyperHeap.root
 
-type uint32_t = UInt32.t
-type uint8_t = UInt8.t
+module U32 = FStar.UInt32
+module U8 = FStar.UInt8
+type uint32_t = U32.t
+type uint8_t = U8.t
 
 let hash_size = 32
-type hash = b:B.buffer uint8_t{B.length b = hash_size}
+// type hash = b:B.buffer uint8_t{B.length b = hash_size}
+type hash = b:B.buffer uint8_t
 let hash_buf = B.buffer hash
 
-// assume val hash_from_hashes: 
-//   src1:hash -> src2:hash -> dst:hash -> 
-//   HST.St unit
-// 	 (requires (fun h0 -> 
-// 	   B.live h0 src1 /\ B.live h0 src2 /\ B.live h0 dst))
-// 	 (ensures (fun h0 _ h1 ->
-// 	   modifies (loc_addr_of_buffer
+assume val hash_from_hashes: 
+  src1:hash -> src2:hash -> dst:hash -> 
+  HST.ST unit
+	 (requires (fun h0 ->
+	   B.live h0 src1 /\ B.live h0 src2 /\ B.live h0 dst))
+	 (ensures (fun h0 _ h1 ->
+	   modifies (loc_buffer dst) h0 h1))
 
-/// Utilities
+/// Power of 2
 
-val uint32_pow2: sz:uint32_t{sz < 32ul} -> Tot uint32_t
-let rec uint32_pow2 sz =
-  UInt32.shift_left 1ul sz
+val uint32_pow2: 
+  sz:uint32_t{sz < 32ul} -> Tot (p:uint32_t{U32.v p = pow2 (U32.v sz)})
+let uint32_pow2 sz =
+  let p = UInt32.shift_left 1ul sz in
+  assume (U32.v p = pow2 (U32.v sz));
+  p
 
-val uint32_is_pow2: uint32_t -> Tot bool
-let rec uint32_is_pow2 n =
-  n <> 0ul && UInt32.logor n (n -% 1ul) = 0ul
+val is_pow2: nat -> GTot bool
+let rec is_pow2 n =
+  if n = 0 then false
+  else if n = 1 then true
+  else (n % 2 = 0 && is_pow2 (n / 2))
+
+val uint32_is_pow2: n:uint32_t -> Tot (b:bool{b = is_pow2 (U32.v n)})
+let uint32_is_pow2 n =
+  let b = n <> 0ul && UInt32.logor n (n -% 1ul) = 0ul in
+  assume (b = is_pow2 (U32.v n));
+  b
+
+val pow2_floor: 
+  n:nat{n > 0} -> GTot (p:nat{pow2 p <= n && n < pow2 (p + 1)})
+let rec pow2_floor n =
+  if n = 1 then 0 else 1 + pow2_floor (n / 2)
 
 val uint32_pow2_floor: n:uint32_t{n > 0ul} -> 
-  Tot (p:uint32_t{p < 32ul && uint32_pow2 p <= n})
-let uint32_pow2_floor n = admit ()
+  Tot (p:uint32_t{
+    p < 32ul && pow2 (U32.v p) <= U32.v n && U32.v n < pow2 (U32.v p + 1) &&
+    pow2_floor (U32.v n) = U32.v p})
+let uint32_pow2_floor n =
+  admit ()
 
-/// Hash pointers
+val pow2_is_pow2:
+  n:nat ->
+  Lemma (is_pow2 (pow2 n))
+	[SMTPat (is_pow2 (pow2 n))]
+let rec pow2_is_pow2 n =
+  if n = 0 then ()
+  else pow2_is_pow2 (n - 1)
 
-// val copy_hash: src:hash -> dst:hash -> HST.St unit
-// let copy_hash src dst =
-//   B.upd dst 0ul (B.index src 0ul)
-//     B.upd (B.index nvs nelts) 0ul (B.index e 0ul);
+val pow2_floor_pow2:
+  p:nat -> 
+  Lemma (pow2_floor (pow2 p) = p)
+	[SMTPat (pow2_floor (pow2 p))]
+let rec pow2_floor_pow2 p =
+  if p = 0 then ()
+  else pow2_floor_pow2 (p - 1)
 
+/// About hash buffer
 
+val copy_hash: 
+  src:hash{B.length src = hash_size} -> dst:hash{B.length dst = hash_size} -> 
+  HST.ST unit
+	 (requires (fun h0 -> 
+	   B.live h0 src /\ B.live h0 dst /\ B.disjoint src dst))
+	 (ensures (fun h0 _ h1 ->
+	   modifies (loc_buffer dst) h0 h1 /\
+	   B.as_seq h1 dst = B.as_seq h0 src))
+let copy_hash src dst =
+  blit src 0ul dst 0ul (U32.uint_to_t hash_size)
+
+val buffer_for_each:
+  #a:Type -> h:HS.mem -> b:B.buffer a -> 
+  prop:(a -> GTot Type0) -> GTot Type0
+let buffer_for_each #a h b prop =
+  forall (i:nat{i < B.length b}). prop (B.get h b i)
+
+val buffer_for_each_gsub:
+  #a:Type -> h:HS.mem -> b:B.buffer a ->
+  prop:(a -> GTot Type0) ->
+  i:uint32_t -> len:uint32_t ->
+  Lemma (requires (B.length b = U32.v len /\ i <= len /\
+		  buffer_for_each h (B.gsub b 0ul i) prop /\
+		  buffer_for_each h (B.gsub b i (len - i)) prop))
+	(ensures (buffer_for_each h b prop))
+let buffer_for_each_gsub #a h b prop i len =
+  admit ()
+
+val hash_buf_allocated: 
+  h:HS.mem -> hs:hash_buf -> GTot Type0
+let hash_buf_allocated h hs =
+  buffer_for_each h hs
+  (fun hb -> B.live h hb /\ B.length hb = hash_size)
+
+val hash_buf_allocated_gsub:
+  h:HS.mem -> hs:hash_buf ->
+  i:uint32_t -> len:uint32_t ->
+  Lemma (requires (B.length hs = U32.v len /\ i <= len /\
+		  hash_buf_allocated h (B.gsub hs 0ul i) /\
+		  hash_buf_allocated h (B.gsub hs i (len - i))))
+	(ensures (hash_buf_allocated h hs))
+	[SMTPat (hash_buf_allocated h (B.gsub hs 0ul i));
+	SMTPat (hash_buf_allocated h (B.gsub hs i (len - i)))]
+let hash_buf_allocated_gsub h hs i len =
+  buffer_for_each_gsub h hs 
+  (fun hb -> B.live h hb /\ B.length hb = hash_size)
+  i len
+
+/// Allocation by power of two
+
+val alloc_sz_lg:
+  nelts:nat{nelts > 0} -> 
+  GTot (sz:nat{sz > 0 && pow2 (sz - 1) <= nelts && nelts < pow2 sz})
+let rec alloc_sz_lg nelts = pow2_floor nelts + 1
+
+unfold val alloc_sz: nelts:nat -> GTot nat
+unfold let alloc_sz nelts =
+  if nelts = 0 then 0
+  else pow2 (alloc_sz_lg nelts) - 1
+
+val alloc_sz_lg_pow2_inc:
+  nelts:nat{nelts > 0} ->
+  Lemma (requires (is_pow2 (nelts + 1)))
+	(ensures (alloc_sz_lg (nelts + 1) = 1 + alloc_sz_lg nelts))
+let rec alloc_sz_lg_pow2_inc nelts =
+  if nelts = 1 then ()
+  else alloc_sz_lg_pow2_inc (nelts / 2)
+
+val alloc_sz_lg_not_pow2_inc:
+  nelts:nat{nelts > 0} ->
+  Lemma (requires (~ (is_pow2 (nelts + 1))))
+	(ensures (alloc_sz_lg nelts = alloc_sz_lg (nelts + 1)))
+let alloc_sz_lg_not_pow2_inc nelts =
+  let sz1 = alloc_sz_lg nelts in
+  let sz2 = alloc_sz_lg (nelts + 1) in
+  if sz1 > sz2 
+  then Math.Lemmas.pow2_le_compat (sz1 - 1) sz2
+  else if sz1 < sz2
+  then (Math.Lemmas.pow2_le_compat (sz2 - 1) sz1;
+       assert (nelts = pow2 sz1))
+  else ()
 
 /// Low-level Merkle tree data structure
 
 noeq type merkle_tree =
-| MT: nelts:uint32_t{nelts > 0ul} -> 
+| MT: nelts:uint32_t ->
       // The value buffer will be resized when elements are added.
       // Resizing mechanism will be similar to that of C++ vector.
-      values:hash_buf ->
+      values_sz:uint32_t{values_sz >= nelts} ->
+      values:hash_buf{B.length values = U32.v values_sz} ->
       // The actual number of internal roots should be equal to 
       // the number of "set" bits of `nelts`.
-      iroots:hash_buf ->
+      iroots:hash_buf{B.length iroots = U32.n} ->
       merkle_tree
 
-let mtree_ptr = B.pointer merkle_tree
+let mt_ptr = B.pointer merkle_tree
 
 /// Initialization
 
+val create_hashes:
+  len:uint32_t{len > 0ul} ->
+  HST.ST hash_buf
+	 (requires (fun h0 -> true))
+	 (ensures (fun h0 hs h1 ->
+	   B.unused_in hs h0 /\ B.live h1 hs /\
+	   B.length hs = U32.v len /\
+	   modifies (loc_buffer hs) h0 h1 /\
+	   B.freeable hs))
+let create_hashes len = 
+  B.malloc root B.null len
 
-
-val create_hashes: 
-  idx:uint32_t -> len:uint32_t -> 
-  hs:B.buffer hash{UInt32.v idx < B.length hs} ->
+val init_hashes: 
+  len:uint32_t -> hs:hash_buf{B.length hs = U32.v len} ->
   HST.ST unit
 	 (requires (fun h0 -> B.live h0 hs))
-	 (ensures (fun h0 _ h1 -> modifies (loc_buffer hs) h0 h1))
-let rec create_hashes idx len hs =
+	 (ensures (fun h0 _ h1 ->
+	   hash_buf_allocated h1 hs /\
+	   B.live h1 hs /\ 
+	   modifies (loc_buffer hs) h0 h1))
+#set-options "--z3rlimit 10"
+let rec init_hashes len hs =
   if len = 0ul then ()
-  else (B.upd hs idx (B.malloc root (UInt8.uint_to_t 0) hash_size);
-       assume (UInt32.v (idx + 1ul) < B.length hs);
-       create_hashes (idx + 1ul) (len - 1ul) hs)
+  else (B.upd hs 0ul (B.malloc root (UInt8.uint_to_t 0) (U32.uint_to_t hash_size));
+       init_hashes (len - 1ul) (B.sub hs 1ul (len - 1ul));
+       let hh = HST.get () in
+       assert (hash_buf_allocated hh (B.gsub hs 0ul 1ul)))
+
+val init_hashes_partial:
+  idx:uint32_t -> len:uint32_t -> 
+  hs:hash_buf{U32.v idx + U32.v len <= B.length hs} ->
+  HST.ST unit
+	 (requires (fun h0 -> B.live h0 hs))
+	 (ensures (fun h0 _ h1 ->
+	   hash_buf_allocated h1 (B.gsub hs idx len) /\
+	   B.live h1 hs /\ 
+	   modifies (loc_buffer (B.gsub hs idx len)) h0 h1))
+let rec init_hashes_partial idx len hs =
+  init_hashes len (B.sub hs idx len)
 
 val create_merkle_tree: unit -> 
-  HST.ST mtree_ptr
+  HST.ST mt_ptr
 	 (requires (fun _ -> true))
 	 (ensures (fun h0 mt h1 -> true))
 let create_merkle_tree _ = 
-  let values = B.malloc root B.null 1ul in
-  create_hashes 0ul 1ul values;
-  let iroots = B.malloc root B.null 32ul in
-  create_hashes 0ul 32ul iroots;
-  B.malloc root (MT 1ul values iroots) 1ul
+  let values = B.null in
+  let iroots = create_hashes 32ul in
+  init_hashes 32ul iroots;
+  B.malloc root (MT 0ul 0ul values iroots) 1ul
 
 /// Insertion
 
 val insert_values:
-  nelts:uint32_t{nelts > 0ul} -> 
-  vs:hash_buf ->
-  e:hash -> 
+  nelts:uint32_t{U32.v nelts < UInt.max_int U32.n} ->
+  nvs:uint32_t{nvs >= nelts && U32.v nvs <= UInt.max_int U32.n} ->
+  vs:hash_buf{B.length vs = U32.v nvs} ->
+  e:hash{B.length e = hash_size} -> 
   HST.ST (ivs:hash_buf)
-	 (requires (fun h0 -> B.live h0 vs /\ B.freeable vs))
-	 (ensures (fun h0 nvs h1 -> B.live h1 nvs /\ B.freeable nvs))
-#set-options "--z3rlimit 10"
-let insert_values nelts vs e =
-  if uint32_is_pow2 (nelts +% 1ul)
-  then (let nvs = B.malloc root B.null (2ul * (nelts + 1ul)) in
-       // `blit` requires two buffers to be disjoint
-       LowStar.BufferOps.blit vs 0ul nvs 0ul nelts;
-       create_hashes (nelts + 1ul) (nelts + 1ul) nvs;
-       B.upd (B.index nvs nelts) 0ul (B.index e 0ul);
-
-       B.free vs;
-       let hh2 = HST.get () in assume (B.live hh2 nvs);
-       nvs)
-  else (assume (UInt32.v nelts < B.length vs);
-       B.upd vs nelts e; vs)
+	 (requires (fun h0 -> B.live h0 e /\ B.live h0 vs /\ B.freeable vs))
+	 (ensures (fun h0 ivs h1 -> B.live h1 ivs /\ B.freeable ivs))
+// #set-options "--z3rlimit 10"
+let insert_values nelts nvs vs e =
+  // if nelts = nvs 
+  // then (assume (2 * U32.v nelts + 1 <= UInt.max_int U32.n);
+  //      let ivs = create_hashes (2ul * nelts + 1ul) in
+  //      LowStar.BufferOps.blit vs 0ul ivs 0ul nelts;
+  //      init_hashes_partial nelts (nelts + 1ul) ivs;
+  //      copy_hash e (B.index ivs nelts);
+  //      B.free vs;
+  //      let hh2 = HST.get () in assume (B.live hh2 ivs);
+  //      ivs)
+  // else admit ()
+  admit ()
 
 val num_iroots_of: nelts:uint32_t -> Tot uint32_t
 let rec num_iroots_of nelts =
@@ -138,40 +278,39 @@ val insert_iroots:
 	 (ensures (fun h0 _ h1 -> true))
 #set-options "--z3rlimit 20"
 let rec insert_iroots nelts irs nv =
-  if nelts = 1ul
-  then (assume (B.length irs > 0);
-       hash_from_hashes (B.index irs 0ul) nv (B.index irs 0ul))
-  else if uint32_is_pow2 nelts
-  then B.upd (B.index irs 1ul) 0ul (B.index nv 0ul)
-  else (insert_iroots (nelts -% uint32_pow2 (uint32_pow2_floor nelts))
-  		      (B.sub irs 1ul (num_iroots_of nelts - 1))
-  		      nv;
-       if nelts +% 1ul = uint32_pow2 (uint32_pow2_floor nelts +% 1ul)
-       then hash_from_hashes (B.index irs 0ul) (B.index irs 1ul) 
-       			     (B.index irs 0ul)
-       else ())
-
+  // if nelts = 1ul
+  // then (assume (B.length irs > 0);
+  //      hash_from_hashes (B.index irs 0ul) nv (B.index irs 0ul))
+  // else if uint32_is_pow2 nelts
+  // then B.upd (B.index irs 1ul) 0ul (B.index nv 0ul)
+  // else (insert_iroots (nelts -% uint32_pow2 (uint32_pow2_floor nelts))
+  // 		      (B.sub irs 1ul (num_iroots_of nelts - 1))
+  // 		      nv;
+  //      if nelts +% 1ul = uint32_pow2 (uint32_pow2_floor nelts +% 1ul)
+  //      then hash_from_hashes (B.index irs 0ul) (B.index irs 1ul) 
+  //      			     (B.index irs 0ul)
+  //      else ())
+  admit ()
+  
 val insert: 
-  mt:mtree_ptr -> e:hash -> 
+  mt:mt_ptr -> e:hash -> 
   HST.ST merkle_tree
 	 (requires (fun h0 -> true))
 	 (ensures (fun h0 nmt h1 -> true))
 let insert mt e =
-  let nnelts = insert_nelts (MT?.nelts mt) in
-  let niroots = insert_iroots (MT?.nelts mt) (MT?.iroots mt) e; MT?.iroots mt in
-  let nvalues = insert_values (MT?.nelts mt) (MT?.values mt) e in
+  // let nnelts = insert_nelts (MT?.nelts mt) in
+  // let niroots = insert_iroots (MT?.nelts mt) (MT?.iroots mt) e; MT?.iroots mt in
+  // let nvalues = insert_values (MT?.nelts mt) (MT?.values mt) e in
   admit () // MT nnelts nvalues niroots
 
 /// Getting the Merkle root
 
 val merkle_root_of_iroots:
-  nirs:nat{nirs <= max_nelts_sz} ->
-  irs:hash_buf{B.length irs = max_nelts_sz} -> 
+  nirs:nat{nirs <= U32.n} ->
+  irs:hash_buf{B.length irs = U32.n} -> 
   HST.ST hash
 	 (requires (fun h0 -> B.live h0 irs))
-	 (ensures (fun h0 hs h1 -> 
-	   h1 == h0 /\
-	   High.merkle_root_of_iroots (B.as_seq h0 irs) = hs))
+	 (ensures (fun h0 hs h1 -> h1 == h0))
 let merkle_root_of_iroots nirs irs =
   admit ()
 
